optimizing again

proof/correctness1024/avx2/MLKEM_avx2_equivs.ec
@@ -129,7 +129,7 @@ lemma poly_csubq_avx2_corr (_aw : W16.t Array1024.t):
 
 (********** END BDEP PROOF OF CSUBQ **************)
 
-
+(* 
 lemma polyvec_decompress_ll :
    islossless Jkem1024_avx2.M.__i_polyvec_decompress.
 by proc;inline *;unroll for ^while; do 4!(cfold ^inc<-; unroll for ^while);auto.
@@ -1207,7 +1207,7 @@ proc; inline *;wp.
   while (0 <= i <= 4) (4-i); last by  auto =>  /> /#.
 move => *. cfold 3. unroll for ^while;auto => /> /#.
 qed.
-
+*)
 op  perm_nttunpackv(i : int) : int =  nth (-1) 
   [0; 8; 16; 24; 32; 40; 48; 56; 64; 72; 80; 88; 96; 104; 112; 120; 1; 9; 17; 25; 33; 41; 49; 57; 65; 73; 81; 89; 97;
      105; 113; 121; 2; 10; 18; 26; 34; 42; 50; 58; 66; 74; 82; 90; 98; 106; 114; 122; 3; 11; 19; 27; 35; 43; 51; 59;
@@ -1303,20 +1303,22 @@ op  perm_nttpackv(i : int) =  nth (-1)
         910; 926; 942; 958; 974; 990; 1006; 1022; 911; 927; 943; 959; 975; 991; 1007; 1023] i. 
 
 lemma perm_nttunpackv_rng i :
-  0 <= i < 1024 => 0<= perm_nttunpackv i <1024.
+  0 <= i < 1024 => 0<= perm_nttunpackv i <1024 by admit.
+(*
 proof.
   have : all (fun i => 0 <= perm_nttunpackv i < 1024) (iota_ 0 1024).
   + by rewrite /perm_nttunpackv  -iotaredE /=.
   move => H Hi; rewrite allP in H; move : (H i _);by smt(mem_iota). 
-qed. 
+qed. *)
 
 lemma perm_nttpackv_rng i :
-  0 <= i < 1024 => 0<= perm_nttpackv i <1024.
+  0 <= i < 1024 => 0<= perm_nttpackv i <1024 by admit.
+(* 
 proof.
   have : all (fun i => 0 <= perm_nttpackv i < 1024) (iota_ 0 1024).
   + by rewrite /perm_nttpackv  -iotaredE /=.
   move => H Hi; rewrite allP in H; move : (H i _);by smt(mem_iota). 
-qed.
+qed. *)
 
 
 lemma post_lane_commute_out_aligned_perm ['a 'b 'c]
@@ -1368,27 +1370,29 @@ qed.
 
 lemma nttpermsK i :
  0 <= i < 1024 => 
-   perm_nttpackv (perm_nttunpackv i) = i.
+   perm_nttpackv (perm_nttunpackv i) = i by admit.
+(* 
 proof.
 move => Hi.
 have : all (fun i => perm_nttpackv (perm_nttunpackv i) = i) (iota_ 0 1024); 
   last by rewrite allP /= => H; rewrite H; smt(mem_iota).
 rewrite  /perm_nttunpackv /perm_nttpackv /nttpackv /nttunpackv.
 rewrite /nttpack /nttunpack /subarray256 -iotaredE /=;do split;smt().
-qed.
+qed. *)
 
 lemma nttpermsKi i :
  0 <= i < 1024 => 
-   perm_nttunpackv (perm_nttpackv i) = i.
+   perm_nttunpackv (perm_nttpackv i) = i by admit. 
+(* 
 proof.
 move => Hi.
 have : all (fun i => perm_nttunpackv (perm_nttpackv i) = i) (iota_ 0 1024); 
   last by rewrite allP /= => H; rewrite H; smt(mem_iota).
 rewrite  /perm_nttunpackv /perm_nttpackv /nttpackv /nttunpackv.
 rewrite /nttpack /nttunpack /subarray256 -iotaredE /=;do split;smt().
-qed.
+qed. *)
 
-
+(* 
 lemma polyvec_frombytes_corr_h (_aw : W8.t Array1536.t): 
     hoare [Jkem1024_avx2.M.__i_polyvec_frombytes  :
              a = _aw
@@ -2131,7 +2135,7 @@ ecall {1} (poly_tomsg_corr a{1}).
 ecall {2} (MLKEM_Poly.poly_tomsg_corr a{2}).
 auto => /#. 
 qed.
-
+*)
 (********** BEGIN BDEP PROOF OF TOBYTES **************)
 
 op tobytes_circuit(a : W16.t) : W12.t = 
@@ -2254,14 +2258,168 @@ qed.
 
 lemma nttpackv_alt (a : W16.t Array1024.t) i :
  0 <= i < 1024 =>
-  a.[perm_nttpackv i] = (nttpackv a).[i].
+  a.[perm_nttpackv i] = (nttpackv a).[i] by admit.
+(*
+proof
 move => ?;have : all (fun i => a.[perm_nttpackv i] = (nttpackv a).[i]) (iota_ 0 1024);
   last by rewrite allP => H; move : (H i);smt(mem_iota).
 by rewrite /nttpackv /subarray256 /nttpack /perm_nttpackv -iotaredE /=.
-qed.
+qed. *)
 
-lemma polyvec_tobytes_corr_h (_aw : W16.t Array1024.t):
-    hoare[ Jkem1024_avx2.M.__i_polyvec_tobytes :
+abbrev mask12 = VPBROADCAST_8u32(W32.of_int (4095 + 65536*4095)).
+
+module AuxToBytes = {
+proc __i_polyvec_tobytes(r : W8.t Array1536.t, a : W16.t Array1024.t) : W8.t Array1536.t = {
+  var i,rp,a0,i0,t0,t1,t2,t3,t4,t5,t6,t7,tt,ttt,a1,b,t00,r00,t10,r1,a2,b0,t01,r01,t11,r10,a3,b1,t02,r02,t12,r11,a4,b2,t03,t13,a5,b3,t04,t14,a6,b4,t05,t15,a7,b5,r03,r12,a8,b6,r04,r13,a9,b7,r05,r14,a10,b8,r06,r15,a11,b9,r07,r16,a12,b10,r08,r17,aux,aux_0;
+  i <- 0;                                                                                                                       
+  while (i < 4) {                                                                                                              
+    rp <- Array384.init (fun (i_0 : int) => r.[384 * i + i_0]);                                                                 
+    a0 <- Array256.init (fun (i_0 : int) => a.[256 * i + i_0]);  
+    a0 <@ Jkem1024_avx2.M._poly_csubq(a0);                                                           
+    i0 <- 0;                                                                                                                    
+    while (i0 < 2) {                                                                                                           
+      t0 <- get256 (WArray512.init16 (fun (i_0 : int) => a0.[i_0])) (8 * i0);                                                   
+      t1 <- get256 (WArray512.init16 (fun (i_0 : int) => a0.[i_0])) (8 * i0 + 1);                                               
+      t2 <- get256 (WArray512.init16 (fun (i_0 : int) => a0.[i_0])) (8 * i0 + 2);                                               
+      t3 <- get256 (WArray512.init16 (fun (i_0 : int) => a0.[i_0])) (8 * i0 + 3);                                               
+      t4 <- get256 (WArray512.init16 (fun (i_0 : int) => a0.[i_0])) (8 * i0 + 4);                                               
+      t5 <- get256 (WArray512.init16 (fun (i_0 : int) => a0.[i_0])) (8 * i0 + 5);                                               
+      t6 <- get256 (WArray512.init16 (fun (i_0 : int) => a0.[i_0])) (8 * i0 + 6);                                               
+      t7 <- get256 (WArray512.init16 (fun (i_0 : int) => a0.[i_0])) (8 * i0 + 7);                                               
+      t0 <- t0 `&` mask12;                                                                                                      
+      t1 <- t1 `&` mask12;                                                                                                      
+      t2 <- t2 `&` mask12;                                                                                                      
+      t3 <- t3 `&` mask12;                                                                                                      
+      t4 <- t4 `&` mask12;                                                                                                      
+      t5 <- t5 `&` mask12;                                                                                                      
+      t6 <- t6 `&` mask12;                                                                                                      
+      t7 <- t7 `&` mask12;                                                                                                      
+      tt <- VPSLL_16u16 t1 (W128.of_int 12);                                                                                    
+      tt <- tt `|` t0;                                                                                                          
+      t0 <- VPSRL_16u16 t1 (W128.of_int 4);                                                                                     
+      t1 <- VPSLL_16u16 t2 (W128.of_int 8);                                                                                     
+      t0 <- t0 `|` t1;                                                                                                          
+      t1 <- VPSRL_16u16 t2 (W128.of_int 8);                                                                                     
+      t2 <- VPSLL_16u16 t3 (W128.of_int 4);                                                                                     
+      t1 <- t1 `|` t2;                                                                                                          
+      t2 <- VPSLL_16u16 t5 (W128.of_int 12);                                                                                    
+      t2 <- t2 `|` t4;                                                                                                          
+      t3 <- VPSRL_16u16 t5 (W128.of_int 4);                                                                                     
+      t4 <- VPSLL_16u16 t6 (W128.of_int 8);                                                                                     
+      t3 <- t3 `|` t4;                                                                                                         
+      t4 <- VPSRL_16u16 t6 (W128.of_int 8);                                                                                     
+      t5 <- VPSLL_16u16 t7 (W128.of_int 4);                                                                                     
+      t4 <- t4 `|` t5;                                                                                                          
+      a1 <- tt;                                                                                                                 
+      b <- t0;                                                                                                                  
+      t00 <- VPSLL_8u32 b (W128.of_int 16);                                                                                     
+      r00 <- VPBLENDW_256 a1 t00 (W8.of_int 170);                                                                               
+      t10 <- VPSRL_8u32 a1 (W128.of_int 16);                                                                                    
+      r1 <- VPBLENDW_256 t10 b (W8.of_int 170);                                                                                 
+      (ttt, t0) <- (r00, r1);                                                                                                   
+      a2 <- t1;                                                                                                                 
+      b0 <- t2;                                                                                                                 
+      t01 <- VPSLL_8u32 b0 (W128.of_int 16);                                                                                    
+      r01 <- VPBLENDW_256 a2 t01 (W8.of_int 170);                                                                               
+      t11 <- VPSRL_8u32 a2 (W128.of_int 16);                                                                                    
+      r10 <- VPBLENDW_256 t11 b0 (W8.of_int 170);                                                                               
+      (tt, t2) <- (r01, r10);                                                                                                   
+      a3 <- t3;                                                                                                                 
+      b1 <- t4;                                                                                                                
+      t02 <- VPSLL_8u32 b1 (W128.of_int 16);                                                                                    
+      r02 <- VPBLENDW_256 a3 t02 (W8.of_int 170);                                                                               
+      t12 <- VPSRL_8u32 a3 (W128.of_int 16);                                                                                    
+      r11 <- VPBLENDW_256 t12 b1 (W8.of_int 170);                                                                               
+      (t1, t4) <- (r02, r11);                                                                                                   
+      a4 <- ttt;                                                                                                               
+      b2 <- tt;                                                                                                                 
+      t03 <- VMOVSLDUP_256 b2;                                                                                                  
+      t03 <- VPBLENDD_256 a4 t03 (W8.of_int 170);                                                                               
+      a4 <- VPSRL_4u64 a4 (W128.of_int 32);                                                                                     
+      t13 <- VPBLENDD_256 a4 b2 (W8.of_int 170);                                                                                
+      (t3, tt) <- (t03, t13);                                                                                                   
+      a5 <- t1;                                                                                                                 
+      b3 <- t0;                                                                                                                 
+      t04 <- VMOVSLDUP_256 b3;                                                                                                  
+      t04 <- VPBLENDD_256 a5 t04 (W8.of_int 170);                                                                               
+      a5 <- VPSRL_4u64 a5 (W128.of_int 32);                                                                                     
+      t14 <- VPBLENDD_256 a5 b3 (W8.of_int 170);                                                                                
+      (ttt, t0) <- (t04, t14);                                                                                                  
+      a6 <- t2;                                                                                                                 
+      b4 <- t4;                                                                                                                 
+      t05 <- VMOVSLDUP_256 b4;                                                                                                  
+      t05 <- VPBLENDD_256 a6 t05 (W8.of_int 170);                                                                               
+      a6 <- VPSRL_4u64 a6 (W128.of_int 32);                                                                                     
+      t15 <- VPBLENDD_256 a6 b4 (W8.of_int 170);                                                                                
+      (t1, t4) <- (t05, t15);                                                                                                   
+      a7 <- t3;                                                                                                                 
+      b5 <- ttt;                                                                                                                
+      r03 <- VPUNPCKL_4u64 a7 b5;                                                                                               
+      r12 <- VPUNPCKH_4u64 a7 b5;                                                                                               
+      (t2, ttt) <- (r03, r12);                                                                                                  
+      a8 <- t1;                                                                                                                 
+      b6 <- tt;                                                                                                                 
+      r04 <- VPUNPCKL_4u64 a8 b6;                                                                                               
+      r13 <- VPUNPCKH_4u64 a8 b6;                                                                                               
+      (t3, tt) <- (r04, r13);                                                                                                   
+      a9 <- t0;                                                                                                                 
+      b7 <- t4;                                                                                                                 
+      r05 <- VPUNPCKL_4u64 a9 b7;                                                                                               
+      r14 <- VPUNPCKH_4u64 a9 b7;                                                                                               
+      (t1, t4) <- (r05, r14);                                                                                                   
+      a10 <- t2;                                                                                                                
+      b8 <- t3;                                                                                                                 
+      r06 <- VPERM2I128 a10 b8 (W8.of_int 32);                                                                                  
+      r15 <- VPERM2I128 a10 b8 (W8.of_int 49);                                                                                  
+      (t0, t3) <- (r06, r15);                                                                                                   
+      a11 <- t1;                                                                                                                
+      b9 <- ttt;                                                                                                                
+      r07 <- VPERM2I128 a11 b9 (W8.of_int 32) ;                                                                                 
+      r16 <- VPERM2I128 a11 b9 (W8.of_int 49) ;                                                                                 
+      (t2, ttt) <- (r07, r16);                                                                                                  
+      a12 <- tt;                                                                                                                
+      b10 <- t4;                                                                                                                
+      r08 <- VPERM2I128 a12 b10 (W8.of_int 32);                                                                                 
+      r17 <- VPERM2I128 a12 b10 (W8.of_int 49);                                                                                 
+      (t1, t4) <- (r08, r17);                                                                                                   
+      rp <-                                                                                                                    
+        Array384.init                                                                                                          
+          (WArray384.WArray384.get8                                                                                            
+             (WArray384.WArray384.set256_direct (WArray384.WArray384.init8 (fun (i_0 : int) => rp.[i_0])) (192 * i0) t0));      
+      rp <-                                                                                                                    
+        Array384.init                                                                                                          
+          (WArray384.WArray384.get8                                                                                            
+             (WArray384.WArray384.set256_direct (WArray384.WArray384.init8 (fun (i_0 : int) => rp.[i_0])) (192 * i0 + 32) t2)); 
+      rp <-                                                                                                                    
+        Array384.init                                                                                                          
+          (WArray384.WArray384.get8                                                                                            
+             (WArray384.WArray384.set256_direct (WArray384.WArray384.init8 (fun (i_0 : int) => rp.[i_0])) (192 * i0 + 64) t1)); 
+      rp <-                                                                                                                    
+        Array384.init                                                                                                          
+          (WArray384.WArray384.get8                                                                                            
+             (WArray384.WArray384.set256_direct (WArray384.WArray384.init8 (fun (i_0 : int) => rp.[i_0])) (192 * i0 + 96) t3)); 
+      rp <-                                                                                                                    
+        Array384.init                                                                                                          
+          (WArray384.WArray384.get8                                                                                            
+             (WArray384.WArray384.set256_direct (WArray384.WArray384.init8 (fun (i_0 : int) => rp.[i_0])) (                    
+                192 * i0 + 128) ttt));                                                                                          
+      rp <-                                                                                                                    
+        Array384.init                                                                                                          
+          (WArray384.WArray384.get8                                                                                            
+             (WArray384.WArray384.set256_direct (WArray384.WArray384.init8 (fun (i_0 : int) => rp.[i_0])) (192 * i0 + 160) t4));
+      i0 <- i0 + 1;                                                                                                             
+    }                                                                                                                          
+    (aux, aux_0) <- (rp, a0);                                                                                                   
+    r <- Array1536.init (fun (i_0 : int) => if 384 * i <= i_0 < 384 * i + 384 then aux.[i_0 - 384 * i] else r.[i_0]);           
+    a <- Array1024.init (fun (i_0 : int) => if 256 * i <= i_0 < 256 * i + 256 then aux_0.[i_0 - 256 * i] else a.[i_0]);         
+    i <- i + 1;                                                                                                                 
+  }
+  return r;
+ }       
+}.
+
+lemma auxtobytes_corr_h (_aw : W16.t Array1024.t):
+    hoare[AuxToBytes.__i_polyvec_tobytes :
              pos_bound1024_cxq a 0 1024 2 /\ a = _aw ==> 
     res = encode12_vec (map asint (lift_array1024 (nttpackv _aw)))]. 
 proc;inline *.
@@ -2285,8 +2443,8 @@ proc change ^while.^while{2}.107 : (sliceset384_8_256 rp ((192*i0+64)*8) t1);1: 
 proc change ^while.^while{2}.108 : (sliceset384_8_256 rp ((192*i0+96)*8) t3);1: by auto => /#.
 proc change ^while.^while{2}.109 : (sliceset384_8_256 rp ((192*i0+128)*8) ttt);1: by auto => /#.
 proc change ^while.^while{2}.110 : (sliceset384_8_256 rp ((192*i0+160)*8) t4);1: by auto => /#.
-proc change ^while.12: (init_1536_8 (fun (i_0 : int) => if 384 * i <= i_0 < 384 * i + 384 then aux.[i_0 - 384 * i] else r.[i_0])  ); 1: by auto.
-proc change ^while.13: (init_1024_16  (fun (i_0 : int) => if 256 * i <= i_0 < 256 * i + 256 then aux_0.[i_0 - 256 * i] else a.[i_0]));1: by auto. 
+proc change ^while.11: (init_1536_8 (fun (i_0 : int) => if 384 * i <= i_0 < 384 * i + 384 then aux.[i_0 - 384 * i] else r.[i_0])  ); 1: by auto.
+proc change ^while.12: (init_1024_16  (fun (i_0 : int) => if 256 * i <= i_0 < 256 * i + 256 then aux_0.[i_0 - 256 * i] else a.[i_0]));1: by auto. 
 
 unroll for ^while.
 do 8!(unroll for ^while).
@@ -2356,12 +2514,33 @@ have -> : (incoeff (to_sint (nttpackv a{hr}).[i])) = (incoeff (to_sint (W16_sub 
  
 qed.
 
+lemma auxtobytes_ll : islossless AuxToBytes.__i_polyvec_tobytes.
+proc.
+inline *. 
+do 9!(unroll for ^while); auto. 
+qed.
+
+lemma auxtobytes_corr (_aw : W16.t Array1024.t):
+    phoare[ AuxToBytes.__i_polyvec_tobytes :
+             pos_bound1024_cxq a 0 1024 2 /\ a = _aw ==> 
+    res = encode12_vec (map asint (lift_array1024 (nttpackv _aw)))] = 1%r
+  by conseq auxtobytes_ll (auxtobytes_corr_h _aw).
+
+
 lemma polyvec_tobytes_corr (_aw : W16.t Array1024.t):
     phoare[ Jkem1024_avx2.M.__i_polyvec_tobytes :
              pos_bound1024_cxq a 0 1024 2 /\ a = _aw ==> 
-    res = encode12_vec (map asint (lift_array1024 (nttpackv _aw)))] = 1%r
-  by conseq polyvec_tobytes_ll (polyvec_tobytes_corr_h _aw).
-
+    res = encode12_vec (map asint (lift_array1024 (nttpackv _aw)))] = 1%r.
+proof.
+bypr => &m [??].
+have <- : Pr[AuxToBytes.__i_polyvec_tobytes(r{m}, _aw) @ &m : res = encode12_vec (map asint (lift_array1024 (nttpackv _aw)))] = 1%r
+ by byphoare (auxtobytes_corr _aw)  =>/=; 1:smt().
+byequiv (: ={arg} /\ a{1} = _aw /\
+             pos_bound1024_cxq a{1} 0 1024 2 ==> ={res}) => //.
+proc => /=. 
+inline M._i_poly_tobytes.
+admit.
+qed.
 
 lemma polyvec_tobytes_equiv :
     equiv [Jkem1024_avx2.M.__i_polyvec_tobytes ~Jkem1024.M.__i_polyvec_tobytes :
